partial work on SP correctness

examples/graph/theories/SPProofs.v
@@ -11,14 +11,16 @@ Require Import DeferredFix.
 Require Import GHC.Num.
 Import GHC.Num.Notations.
 Require Import HeapProofs.
-
+Require Import OrdTactic.
+Require Import RealRing.
 
 (* Inductive relation*)
 Section Ind.
 
 Context {a : Type} {b : Type} { gr : Type -> Type -> Type} {Hgraph : Graph.Graph gr} {Hlaw : Graph.LawfulGraph gr}
 {Hnum: GHC.Num.Num b} {Heq: Base.Eq_ b} {HOrd: Base.Ord b} {Hreal: @GHC.Real.Real b Hnum Heq HOrd}
-{Heq': Base.Eq_ a} {HOrd': Base.Ord a} {Herr: Err.Default (b)}.
+{Heq': Base.Eq_ a} {HOrd': Base.Ord a} {Herr: Err.Default (b)}{Hlaw2 : (@WeightedGraphs.LawfulWGraph a b gr Hgraph) } {HEqLaw: Base.EqLaws b} {HOrdLaw: @OrdLaws b Heq HOrd HEqLaw}
+{HorderedRing: @RealRing b Heq HOrd HEqLaw Hnum Hreal}.
 
 Program Instance path_default : Err.Default (Graph.LPath b).
 Next Obligation.
@@ -32,13 +34,13 @@ Definition natNodes_lt (x y : gr a b) := natNodes x < natNodes y.
 
 Definition natNodes_eq (x y : gr a b) := natNodes x = natNodes y.
 (*Definition list_length_lt {a b} (x y : list a) := size x < size y*)
-Definition heap_length_lt (x y : Heap b (Graph.LPath b)) := (Heap.size x) < (Heap.size y).
+Definition heap_length_lt {A} (x y : Heap b A) := (Heap.size x) < (Heap.size y).
  (*list_lsize (toList x) (toList y).*)
 
-Definition bf_measure_heap:=
-  lex _ _ (natNodes_lt) natNodes_eq (heap_length_lt).
+Definition bf_measure_heap {A} :=
+  lex _ _ (natNodes_lt) natNodes_eq (@heap_length_lt A).
 
-Lemma well_founded_bf_measure_heap : well_founded (bf_measure_heap).
+Lemma well_founded_bf_measure_heap : forall A,  well_founded (@bf_measure_heap A).
 Proof.
   intros. eapply WF_lex.
   - apply f_nat_lt_wf.
@@ -49,7 +51,7 @@ Proof.
   - unfold RelationClasses.Symmetric. intros. unfold natNodes_eq in *. omega.
 Qed. 
 
-Instance need_this_for_equations : WellFounded (bf_measure_heap).
+Instance need_this_for_equations : forall A, WellFounded (@bf_measure_heap A).
 Proof.
   unfold WellFounded. apply well_founded_bf_measure_heap.
 Defined.
@@ -253,7 +255,7 @@ Lemma sp_tail_multi: forall s v g,
 Proof.
   intros. destruct s as[r p].
   remember (snd r, fst r) as r'. generalize dependent r. revert p. 
-  induction r' using (well_founded_induction (well_founded_bf_measure_heap)).
+  induction r' using (well_founded_induction (@well_founded_bf_measure_heap _)).
   intros. destruct r' as [q h]. inversion Heqr'; subst. clear Heqr'. destruct r as [g' h].
   rewrite unfold_sp_tail. unfold expand_sp_tail. destruct (Heap.isEmpty h) eqn : E. apply multi_refl.
   destruct (isEmpty g') eqn : GE. simpl. apply multi_refl. destruct (bool_dec (false || false) true) eqn : U.
@@ -278,7 +280,7 @@ Lemma sp_tail_done: forall s v g,
 Proof.
   intros. unfold done. destruct s as[r p].
   remember (snd r, fst r) as r'. generalize dependent r. revert p. 
-  induction r' using (well_founded_induction (well_founded_bf_measure_heap)).
+  induction r' using (well_founded_induction (@well_founded_bf_measure_heap _)).
   intros. destruct r. simpl in Heqr'. destruct r'. inversion Heqr'. subst. clear Heqr'.
   rewrite unfold_sp_tail. unfold expand_sp_tail. destruct h. simpl. reflexivity.
   destruct (isEmpty g0) eqn : E. simpl. assumption.
@@ -298,6 +300,371 @@ Proof.
 Qed.
 
 End Exec.
+
+Require Import GHC.Base.
+
+Section Correct.
+Require Import Data.Graph.Inductive.Internal.RootPath.
+Require Import Helper.
+
+Definition orl {A} (l l': list A) :=
+  match l with
+  | nil => l'
+  | _ => l
+  end.
+
+Lemma findP_app: forall {A} v (l l' : LRTree A),
+  findP v (l ++ l') = orl (findP v l) (findP v l').
+Proof.
+  intros. generalize dependent l'. induction l; intros.
+  - simpl. reflexivity.
+  - simpl. destruct a0. destruct unLPath. apply IHl. destruct l0.
+    destruct (Base.op_zeze__ v n) eqn : E. simpl. reflexivity.
+    apply IHl.
+Qed.
+
+Lemma node_eq: forall (v v' : Node),
+  v == v' = true <-> v = v'.
+Proof.
+  intros. unfold "==". unfold Eq_Char___. unfold op_zeze____. apply N.eqb_eq.
+Qed. 
+
+Ltac unfold_eq H :=
+  unfold "==" in H; unfold Eq_Char___ in H; unfold op_zeze____ in H;
+  try (apply N.eqb_eq in H); try (apply N.eqb_neq in H).
+
+Lemma graph_iff_not_output: forall s g v v',
+  valid s g v ->
+  vIn g v' = true ->
+  findP v' (get_paths s) <> nil <->  (vIn (get_graph s) v' = false).
+Proof.
+  intros. induction H; split; intros; simpl in *.
+  - contradiction. 
+  - rewrite H0 in H1. inversion H1.
+  - inversion H1; subst.
+    + simpl. unfold get_paths in H2. rewrite findP_app in H2. 
+      destruct (findP v' p) eqn : F. simpl in H2. destruct (Base.op_zeze__ v' v0) eqn : E.
+      apply node_eq in E. subst. epose proof (match_remain_some g0 v0 c g' H4). destruct_all.
+      destruct (vIn g' v0) eqn : V. apply H6 in V. destruct_all; contradiction. reflexivity.
+      contradiction. simpl in IHvalid. 
+      rewrite F in IHvalid. pose proof (match_remain_some g0 v0 c g' H4). destruct_all.
+      destruct (vIn g' v') eqn : V. apply H6 in V. destruct_all. 
+      assert (vIn g0 v' = false). apply IHvalid. assumption. auto. rewrite H10 in H8. inversion H8.
+      reflexivity.
+    + simpl. simpl in IHvalid. simpl in H2. assert (g' = g0). erewrite match_remain_none. reflexivity. apply H4.
+      subst. apply IHvalid. assumption. assumption.
+  - inversion H1; subst. simpl in IHvalid. simpl in H2. simpl. rewrite findP_app. destruct (findP v' p) eqn : F.
+    simpl. destruct (v' == v0) eqn : E. intro. inversion H6. apply IHvalid. assumption.
+    pose proof (match_remain_some g0 v0 c g' H4). destruct_all. destruct (vIn g0 v') eqn : V.
+    assert (vIn g' v' = true). apply H6. split. assumption. intro. subst. unfold_eq E. contradiction.
+    rewrite H8 in H2. inversion H2. reflexivity. simpl. intro. inversion H6.
+    simpl in *. apply IHvalid. assumption. assert (g0 = g'). eapply match_remain_none. apply H4. subst.
+    assumption.
+Qed.
+
+Require Import WeightedGraphs.
+
+Lemma graph_subset: forall s s' v g,
+  valid s v g ->
+  valid s' v g ->
+  sp_multi s s' ->
+  (forall u v w, WeIn (get_graph s') u v w -> WeIn (get_graph s) u v w).
+Proof.
+  intros. induction H1. assumption. inversion H1; subst.
+  - remember ((g', mergeAll (h' :: expand d (LP ((v1, d) :: t)) c), p ++ LP ((v1, d) :: t) :: nil)) as s''.
+    rewrite Heqs'' in IHmulti at 2. simpl in IHmulti. simpl. eapply Wmatch_remain_some in H5.
+    destruct_all. apply IHmulti in H2. apply H7 in H2. destruct_all; assumption. eapply v_step. apply H.
+    assumption. eapply multi_valid. eapply v_step. apply H. apply H1. assumption.
+  - eapply match_remain_none in H5. subst. simpl in *. apply IHmulti. eapply v_step. apply H. assumption.
+    eapply multi_valid. eapply v_step. apply H. apply H1. assumption. assumption.
+Qed.
+
+Lemma valid_begins_with_start: forall s g v,
+  valid s g v ->
+  sp_multi (start g v) s.
+Proof.
+  intros. induction H.
+  - constructor.
+  - eapply multi_trans. apply IHvalid.  eapply multi_step. apply H0. apply multi_refl.
+Qed.
+
+Lemma start_in: forall s v g,
+  valid s g v ->
+  vIn g v = true.
+Proof.
+  intros. induction H.
+  - assumption.
+  - assumption.
+Qed.
+
+Lemma graph_subset_start: forall s v (g: gr a b),
+  valid s g v ->
+  (forall u v w, WeIn (get_graph s) u v w -> WeIn g u v w).
+Proof.
+  intros. remember (start g v) as s'.
+  assert (g = get_graph s'). subst; simpl. reflexivity. rewrite H1. eapply graph_subset.
+  subst. apply v_start. eapply start_in. apply H. apply H. subst. apply valid_begins_with_start. apply H.
+  assumption.
+Qed. 
+
+Definition unlabel_path (l : LPath b) : Path := 
+  match l with
+  | LP l' => map fst l'
+  end.
+(*All paths in the heap are valid Wpaths. Then, we can use the equivalent definitions of Wpaths (in terms of 
+  paths anf path_cost, to reason about the paths*)
+
+(*Require Import GHC.Base.
+Import GHC.Num.Notations.
+*)
+
+Lemma expand_preserves_valid: forall (w : Node) (l: LPath b) (l': list Node)
+   (c : Context a b) (u v : Node) (y : b) (g g': gr a b) g'',
+  unlabel_path l = w :: l' ->
+  Wpath g v u (unlabel_path l) y ->
+  match_ w g'' = (Some c, g') ->
+  (forall u v w, WeIn g'' u v w -> WeIn g u v w) -> 
+  (forall h, In h (expand y l c) ->
+  forall x l'', In_Heap (x, l'') h -> 
+  exists b' u', WeIn g w u' b' /\ x == op_zp__ b' y = true /\  Wpath g v u' (unlabel_path l'') x).
+Proof.
+  intros. unfold expand in H2. destruct c. destruct p. destruct p. destruct l.
+  simpl in H3. rewrite in_map_iff in H3. destruct H3. destruct x0. destruct H3. unfold unit in H3.
+  subst. simpl in H4. destruct H4. inversion H3; subst. simpl. simpl in H. rewrite H.  exists b0.
+  exists n0. simpl in H0. rewrite H in H0. assert (WeIn g w n0 b0).  
+  - apply Wmatch_context in H1. destruct_all. subst. apply H2. apply H6. assumption.
+  - split. assumption. split. destruct HEqLaw; apply Eq_refl. 
+    assert (u = w). inversion H0; subst; reflexivity. subst. econstructor. apply H0. apply H4.
+  - destruct H3.
+Qed. 
+
+Lemma heap_path_value: forall s g v x u d t,
+  valid s g v ->
+  In_Heap (x, (LP ((u, d) :: t))) (get_heap s) ->
+  x = d.
+Proof.
+  intros. induction H.
+  - simpl in H0. destruct H0. inversion H0. subst. reflexivity. destruct H0.
+  - inversion H1; subst.
+    + unfold get_heap in H0. rewrite in_heap_mergeAll in H0. rewrite in_heap_unfold in H0.
+      destruct H0.
+      * simpl in IHvalid. apply IHvalid. rewrite in_heap_splitMin. right. apply H0.
+        intro. subst. inversion H4. rewrite <- splitMin_equiv in H4. inversion H4. apply H6. intro.
+        subst. inversion H4.
+      * rewrite in_heap_exists in H0. destruct H0 as [h'']. destruct H0. simpl in H0.
+        destruct c. destruct p0. destruct p0. rewrite in_map_iff in H0. destruct_all. destruct x0.
+        unfold unit in H0. subst. simpl in H5. destruct H5. inversion H0; subst. reflexivity.
+        destruct H0.
+    + simpl in *. apply IHvalid. rewrite in_heap_splitMin. right.
+      apply H0. intro. subst. inversion H4. rewrite <- splitMin_equiv in H4. inversion H4. apply H6.
+      intro. subst. inversion H4.
+Qed. 
+
+Lemma in_heap_wpath: forall s g v x l,
+  valid s g v ->
+  In_Heap (x, l) (get_heap s) ->
+  exists u, Wpath g v u (unlabel_path l) x.
+Proof.
+  intros. generalize dependent l. revert x. induction H; intros.
+  - simpl in H0. destruct H0. inversion H0; subst. simpl. exists v. constructor. assumption.
+    destruct H0.
+  - inversion H0; subst.
+    + unfold get_heap in H1. rewrite in_heap_mergeAll in H1.
+      rewrite in_heap_unfold in H1. destruct H1.
+    * simpl in IHvalid. apply IHvalid. rewrite in_heap_splitMin. right. apply H1. intro. subst.
+      inversion H4. rewrite <- splitMin_equiv in H4.
+    inversion H4; subst. apply H6. intro. subst. simpl in H4. inversion H4.
+    * rewrite in_heap_exists in H1. destruct H1 as [h'']. destruct H1.
+      pose proof (expand_preserves_valid v0 (LP ((v0, d) :: t)) (map fst t) c v0 v d g g' g0 eq_refl). 
+      assert (a' = d). eapply heap_path_value. apply H. simpl.
+      rewrite in_heap_splitMin. left. reflexivity. intro. subst. inversion H4.
+      rewrite <- splitMin_equiv in H4. inversion H4. apply H8. intro. subst. inversion H4.
+      subst.
+      assert (Wpath g v v0 (unlabel_path (LP ((v0, d) :: t))) d). simpl. simpl in IHvalid.
+      specialize (IHvalid d (LP ((v0, d) :: t))). simpl in IHvalid. destruct IHvalid. 
+      rewrite in_heap_splitMin. left. reflexivity. intro. subst. inversion H4.
+      rewrite <- splitMin_equiv in H4. inversion H4; subst. apply H8.
+      intro. subst. inversion H4. assert (A:=H7). apply hd_path in H7. subst. apply A.
+      specialize (H6 H7 H3).
+      assert ((forall (u v : Node) (w : b), WeIn g0 u v w -> WeIn g u v w)). intros.
+      eapply graph_subset_start. apply H. simpl. assumption. specialize (H6 H8 h'' H1 x l H5).
+      destruct H6 as [b']. destruct H6 as [u']. destruct_all.
+      exists u'. assumption.
+    + simpl in *. apply IHvalid. rewrite in_heap_splitMin. right. apply H1. intro. subst. inversion H4.
+      rewrite <- splitMin_equiv in H4. inversion H4. apply H6. intro. subst. inversion H4.
+Qed.
+
+Lemma in_output_wpath: forall s v g l,
+  valid s g v ->
+  In l (get_paths s) ->
+  exists x u, Wpath g v u (unlabel_path l) x.
+Proof.
+  intros.
+  induction H; subst.
+  - simpl in H0. destruct H0.
+  - inversion H1; subst.
+    + unfold get_paths in H0. apply in_app_or in H0. destruct H0. apply IHvalid. apply H0.
+      simpl in H0. destruct H0. subst. exists a'.   eapply in_heap_wpath. apply H. simpl. rewrite in_heap_splitMin.
+      left. reflexivity. intro. subst. inversion H4. rewrite <- splitMin_equiv in H4. inversion H4. apply H5.
+      intro. subst. inversion H4. destruct H0.
+    + apply IHvalid. simpl in *. assumption.
+Qed.
+
+(*
+
+(*Everything on the heap is in the graph*)
+
+
+(*A safe head function that uses a default value so that we don't have to wrap and unwarp options. We know
+  by above that each list in the output is a valid path, so it is not nil*)
+Definition hdDefault {A} (x : A) (l : list A) : A :=
+  match l with
+  | nil => x
+  | h :: t => h
+  end.
+
+Definition get_verts v l := map (hdDefault v) (map unlabel_path l).
+
+Require Import Coq.Lists.SetoidList.
+
+Lemma nodups_output: forall s g v,
+  valid s g v ->
+  NoDup (get_verts v (get_paths s)).
+Proof.
+  intros. induction H.
+  - simpl. unfold get_verts; simpl. constructor.
+  - inversion H0; subst.
+    + simpl. unfold get_verts. unfold map. rewrite map_map. rewrite map_app.
+      simpl.
+      assert (List.map (fun x : LPath b => hdDefault v (unlabel_path x)) p ++ v0 :: nil = 
+      rev (v0 :: rev (List.map (fun x : LPath b => hdDefault v (unlabel_path x)) p))). simpl.
+      rewrite rev_involutive. reflexivity.
+      rewrite H4. rewrite NoDup_NoDupA. apply NoDupA_rev. apply eq_equivalence.
+      constructor. intro. rewrite <- In_InA_equiv in H5. rewrite <- in_rev in H5.
+      assert (vIn g v0 = true). 
+
+  apply SetoiList.NoDupA_rev. simpl.
+
+(*Each vertex appears at most once in the output*)
+Lemma no_dups_output: forall s g v,
+  valid s g v ->
+  NoDup (map fst (get_dists s)).
+Proof.
+  intros. induction H; simpl.
+  - constructor.
+  - inversion H0; subst; simpl in *.
+    rewrite map_app. simpl. assert (map fst d ++ v0 :: nil = rev (v0 :: rev ((map fst d)))).
+    simpl. rewrite rev_involutive. reflexivity.
+    rewrite H3. rewrite NoDup_NoDupA. apply NoDupA_rev. apply eq_equivalence.
+    constructor. intro. rewrite <- In_InA_equiv in H4. rewrite <- in_rev in H4.
+    assert (vIn g v0 = true). eapply queue_in_graph. apply H. simpl. left. reflexivity. 
+    pose proof (graph_iff_not_output _ _ _ _ H H5) as D; simpl in *.
+    apply D in H4. 
+    assert (vIn g0 v0 = true). apply match_in. exists c. exists g'. assumption.
+    rewrite H6 in H4. inversion H4. apply NoDupA_rev. apply eq_equivalence. rewrite <- NoDup_NoDupA.
+    assumption. assumption.
+Qed. 
+  
+
+
+(*Theorem 24.6 in CLRS*)
+Theorem sp_invariant: forall s g v u,
+  valid s g v ->
+  vIn g u = true ->
+  vIn (get_graph s) u = false ->
+  shortest_wpath g u v (getDistance u (get_paths s)).
+Proof.
+  intros. generalize dependent u. generalize dependent H. induction (get_heap s, get_graph s) using (well_founded_induction well_founded_bf_measure_heap).
+  intros. inversion H0; subst.
+  - simpl. unfold getDistance. simpl. simpl in H2. rewrite H2 in H1. inversion H1.
+  - inversion H4; subst.
+    + simpl. unfold getDistance. rewrite findP_app. destruct (N.eq_dec v0 u). subst.
+      destruct (findP u p0) eqn : F. simpl. assert (u == u = true). apply node_eq. reflexivity.
+      rewrite H8. clear H8. 
+  (*Plan
+    - show that shortest path always exists - DONE
+    - prove that the heap contains valid paths to the start vertex - DONE
+    - so there is a shortest path from u to v
+    - then, if a condition holds at the start of a path and doesn't hold at the end, there is a boundary
+      where it doesn/doesnt not hold (may have proved for SCC)
+    - then I have x and y in the CLRS proof
+    - also, may need to prove that u <> v (which should not be hard) - or really just prove for this*)
+  (*Need to know that shortest_wpath is not None*)
+        unfold findP. simpl.
+    + destruct c. destruct p1. destruct p1. simpl in *.
+
+(*Need to reason about distance*)
+Print expand.
+(*Either have additional distance information*)
+Definition path_cost (l :LPath b) : b :=
+  match l with
+  | LP l' => fold_right (fun (x: LNode b) acc => let (_, y) := x in y + acc) #0 l' end.
+
+Print findP.
+
+
+(*Some stuff
+- prove by well founded induction (strong induction)
+ - need to prove that there is a state where previous one found and multisteps (anything on path)
+- ie, if a path is the min chosen in the heap, all previous ones are already there (?)
+*)
+
+
+*)
+End Correct.
+
+Definition expand_dist (d : b) (v : Node) (c: Context a b) :=
+  match c with
+  | (_, _, _, s) => map (fun x : b * Node => let (l,v') := x in unit (_GHC.Num.+_ l d) v') s
+  end.
+
+Equations sp_distance (x : (Heap b Node) * (gr a b)) : list (b * Node) by wf x (@bf_measure_heap Node) :=
+  sp_distance (h, g) :=  if bool_dec ((Heap.isEmpty h) || (Graph.isEmpty g)) true then nil else
+                        match (splitMinT h) as s return ((splitMinT h = s) -> _) with
+                          |Some ((d,v), h') => fun H : (splitMinT h =  Some ((d,v), h')) =>
+                                match (match_ v g) as y return ((match_ v g = y) -> _ ) with
+                                | (Some c, g') => fun H : (match_ v g) = (Some c, g') => (d,v) :: 
+                                      sp_distance (mergeAll (h' :: expand_dist d v c), g')
+                                | (None, g') => fun H: (match_ v g) = (None, g') => sp_distance (h', g')
+                                 end (eq_refl)
+                          | None => fun H : (splitMinT h = None) => Err.patternFailure
+                         end (eq_refl).
+Next Obligation.
+simpl. destruct c. destruct p. destruct p. unfold Base.map. apply lex1. unfold natNodes_lt. eapply match_decr_size.
+symmetry. apply H.
+Defined.
+Next Obligation.
+apply lex2. symmetry. unfold natNodes_eq. eapply match_none_size. apply H. unfold heap_length_lt.
+unfold splitMin in H0. destruct h. simpl in n. contradiction. inversion H0; subst.
+rewrite (mergeAll_size l). simpl. omega.
+Defined.
+
+Definition expand_sp_distance :=
+  fun x : Heap b Node * gr a b =>
+let (h, g) := x in
+if bool_dec (Heap.isEmpty h || isEmpty g) true
+then nil
+else
+ match splitMinT h as s return (splitMinT h = s -> list (b * Node)) with
+ | Some p =>
+     let (p0, h') as p0 return (splitMinT h = Some p0 -> list (b * Node)) := p in
+     let (d, v) as p1 return (splitMinT h = Some (p1, h') -> list (b * Node)) := p0 in
+     fun _ : splitMinT h = Some (d, v, h') =>
+     (let (m, g') as y return (match_ v g = y -> list (b * Node)) := match_ v g in
+      match m as m0 return (match_ v g = (m0, g') -> list (b * Node)) with
+      | Some c =>
+          fun _ : match_ v g = (Some c, g') => (d, v) :: sp_distance (mergeAll (h' :: expand_dist d v c), g')
+      | None => fun _ : match_ v g = (None, g') => sp_distance (h', g')
+      end) eq_refl
+ | None => fun _ : splitMinT h = None => patternFailure
+ end eq_refl.
+
+Lemma unfold_sp_distance : forall x,
+  sp_distance x = expand_sp_distance x.
+Proof.
+    intros. unfold expand_sp_distance. apply sp_distance_elim. reflexivity.
+Qed.
+
 
 (*Prove equivalence with equations version*)
 
@@ -358,7 +725,161 @@ Lemma unfold_dijkstra' : forall x,
   expand_dijkstra' x = dijkstra' x.
 Proof.
   intros. unfold expand_dijkstra'. apply dijkstra'_elim. reflexivity.
-Qed. 
+Qed.
+
+(*Relation of distance to sp. If we take the list returned by disjkstra's and return the length of the path,
+  as well as the head of the list, ew should get the same as the distance*)
+
+Definition labelHead (l: (LPath b)) : (option b * option Node)  :=
+  match l with
+  | LP nil => (None, None)
+  | LP ((x,y) :: tl) => (Some y, Some x) 
+  end.
+Require Import Coq.Wellfounded.Inverse_Image.
+(*
+(*First, we need to know that nil is not in the heap*)
+Lemma nil_notin_heap: forall h g,
+  (forall x, ~In_Heap (x, LP nil) h) ->
+  *)
+
+(*If we calculate the path cost *)
+Lemma distance_sp: forall (h : Heap b (LPath b)) (h' : Heap b Node) (g: gr a b) (Z: forall x, ~In_Heap (x, LP nil) h),
+  map_heap (fun x l => (labelHead l)) h = map_heap (fun x y => (Some x, Some y)) h' ->
+  map labelHead (dijkstra' (h,g)) =
+  map (fun x => (Some (fst x), Some (snd x))) (sp_distance (h', g)).
+Proof.
+  intros. rewrite <- unfold_dijkstra'. rewrite unfold_sp_distance.
+  remember (h,g) as x. generalize dependent g. generalize dependent h. revert h'.
+  induction x using (well_founded_induction (@well_founded_bf_measure_heap _)).
+  - intros. destruct x. inversion Heqx; subst. clear Heqx. unfold expand_dijkstra'.
+    unfold expand_sp_distance.
+    destruct h. simpl. destruct h'. simpl. reflexivity.
+    simpl in H0. inversion H0.
+    destruct h'. simpl in H0. inversion H0. destruct (isEmpty g) eqn : G'.
+    + simpl. reflexivity.
+    + remember (Heap.Node b0 l l0) as h. remember (Heap.Node b1 n l1) as h'.
+      destruct (bool_dec (Heap.isEmpty h || false) true). subst. simpl in e. inversion e.
+      destruct (bool_dec (Heap.isEmpty h' || false) true). subst. simpl in e. inversion e.
+      clear n0. clear n1.
+      destruct (splitMinT h) eqn : Mi. destruct p. destruct p.
+      pose proof map_splitMin. 
+      assert (splitMinT (map_heap (fun (_ : b) (l : LPath b) => labelHead l) h) = Some (b2, labelHead l2, 
+      map_heap (fun (_ : b) (l : LPath b) => labelHead l) h0)).
+      rewrite <- splitMin_equiv in Mi. rewrite <- splitMin_equiv. 
+      assert (h <> Heap.Empty). intro. subst. inversion H2. inversion Mi.
+      erewrite H1. reflexivity. constructor. apply (None, None). apply H2.
+      apply H4. intro. subst. simpl in H2. inversion H2. intro. subst. inversion H2.
+      assert (C := H2).
+      rewrite H0 in H2. destruct (splitMinT h') eqn : Mi'. destruct p. destruct p.
+      assert (splitMinT (map_heap (fun (x : b) (y : Node) => (Some x, Some y)) h') =
+      Some (b3, (Some b3, Some n0), map_heap (fun (x : b) (y : Node) => (Some x, Some y)) h1)).
+      rewrite <- splitMin_equiv. erewrite map_splitMin. reflexivity. constructor. apply (None, None).
+      intro. subst. inversion H3. rewrite <- splitMin_equiv in Mi'. inversion Mi'. reflexivity.
+      intro. subst. inversion H3. intro. subst. simpl in H3. inversion H3. rewrite H2 in H3.
+      inversion H3.  destruct l2. destruct  unLPath.
+      * subst. exfalso. apply (Z b3). rewrite in_heap_splitMin. left. reflexivity. intro. subst. inversion H4.
+        rewrite <- splitMin_equiv in Mi. 
+        assert ((splitMin (Heap.Node b0 l l0)) = (b3, LP nil, h0)). inversion Mi; subst. simpl. reflexivity. apply H4.
+        intro. inversion H4.
+      * destruct l2. simpl in H6. inversion H6. destruct (match_ n1 g) eqn : M. rewrite H9 in M. rewrite M. destruct m.
+        -- remember ((mergeAll (h0 :: expand b3 (LP ((n0, b3) :: unLPath)) c), g0)) as P. rewrite <- HeqP.
+            remember (mergeAll (h1 :: expand_dist b3 n0 c), g0) as P'. simpl.
+           rewrite HeqP. rewrite HeqP'. rewrite <- unfold_dijkstra'. erewrite H. rewrite unfold_sp_distance. reflexivity.
+          apply lex1. eapply match_decr_size. symmetry. apply M. 3 : { reflexivity. }
+          intros. intro. rewrite in_heap_mergeAll in H4. rewrite in_heap_unfold in H4. destruct H4.
+          apply (Z x). rewrite in_heap_splitMin. right. apply H4. intro. subst. inversion H10.
+          rewrite <- splitMin_equiv in Mi. inversion Mi. apply H11. intro. subst. inversion H10.
+          rewrite in_heap_exists in H4. destruct H4 as [h'']. destruct H4. simpl in H4.
+          destruct c. destruct p. destruct p. rewrite in_map_iff in H4. destruct H4. destruct x0.
+          unfold unit in H4.  simpl in H4. destruct H4; subst. simpl in H10. destruct H10. inversion H4. destruct H4.
+          repeat(rewrite map_mergeAll). 
+          assert (
+           (List.map (map_heap (fun (_ : b) (l2 : LPath b) => labelHead l2))
+     (h0 :: expand b3 (LP ((n0, b3) :: unLPath)) c)) =
+        (List.map (map_heap (fun (x : b) (y : Node) => (Some x, Some y))) (h1 :: expand_dist b3 n0 c))).  simpl. unfold expand_dist.
+        destruct c. destruct p. destruct p. rewrite H7. assert (forall l', 
+         List.map (map_heap (fun (_ : b) (l2 : LPath b) => labelHead l2))
+     (map (fun '(l2, v) => unit (_GHC.Num.+_ l2 b3) (LP ((v, _GHC.Num.+_ l2 b3) :: (n0, b3) :: unLPath))) l') =
+      List.map (map_heap (fun (x : b) (y : Node) => (Some x, Some y)))
+     (map (fun x : b * Node => let (l2, v') := x in unit (_GHC.Num.+_ l2 b3) v') l')). { intros. induction l'.
+      simpl. reflexivity. simpl. rewrite IHl'. simpl. destruct a3. reflexivity. } rewrite H4. reflexivity.
+      rewrite H4. reflexivity.
+        -- rewrite <- unfold_dijkstra'. rewrite unfold_sp_distance. erewrite H. reflexivity.
+           apply lex2. unfold natNodes_eq. symmetry. eapply match_none_size. apply M.
+           unfold heap_length_lt. subst. simpl in Mi. inversion Mi; subst. rewrite (mergeAll_size l0).
+           simpl. omega. 3 : { reflexivity. } intros. intro. apply (Z x). rewrite in_heap_splitMin.
+            right. apply H4. intro. subst. inversion H10. rewrite <- splitMin_equiv in Mi. inversion Mi. apply H11.
+          intro. subst. inversion H10. apply H7.
+      * subst. inversion Mi'.
+      * subst. inversion Mi.
+Qed.
+
+(*Now we prove that it has valid paths and weights*)
+Lemma paths_dijkstra: forall h g,
+  map labelHead (dijkstra' (h,g)) = map (fun l => (path_cost (unlabel_path l), snd (labelHead l))) (dijkstra' (h,g
+
+
+apply lex2. symmetry. unfold natNodes_eq. eapply match_none_size. apply H. unfold heap_length_lt.
+unfold splitMin in H0. destruct h. simpl in n. contradiction. inversion H0; subst.
+rewrite (mergeAll_size l4). simpl. omega.
+
+ }
+     (map (fun x : b * Node => let (l2, v') := x in unit (_GHC.Num.+_ l2 b3) v') l')). intros; induction l'.
+      simpl. rewrite H7. reflexivity. simpl. destruct a3. 
+
+
+ induction a0. simpl. rewrite H7. reflexivity.  simpl.
+
+
+
+ simpl. 
+          destruct c. destruct p. destruct p. simpl. 
+          assert (forall l, 
+          map_heap (fun (_ : b) (l2 : LPath b) => labelHead l2)
+  match
+    map (fun '(l2, v) => unit (_GHC.Num.+_ l2 b3) (LP ((v, _GHC.Num.+_ l2 b3) :: (n0, b3) :: unLPath))) l
+  with
+  | nil => h0
+  | h'0 :: hs => merge (merge h0 h'0) (mergeAll hs)
+  end =
+map_heap (fun (x : b) (y : Node) => (Some x, Some y))
+  match map (fun x : b * Node => let (l2, v') := x in unit (_GHC.Num.+_ l2 b3) v') l with
+  | nil => h1
+  | h'0 :: hs => merge (merge h1 h'0) (mergeAll hs)
+  end). { intros. induction l2. simpl. apply H7.
+    
+      unfold map. unfold
+
+ intros;  induction l2 using (well_founded_induction
+                     (wf_inverse_image _ nat _ (@length _)
+                        PeanoNat.Nat.lt_wf_0)). destruct l2. simpl. assumption. simpl. 
+    rewrite map_merge. rewrite map_merge. rewrite map_merge. rewrite map_merge. 
+     rewrite map_mergeAll. rewrite map_mergeAll. destruct l2. simpl.
+      rewrite H7. destruct p. simpl. reflexivity. simpl.
+     
+
+
+
+ reflexivity. subst.  rewrite H7. simpl.
+    simpl.
+
+
+
+ reflexivity. unfold map. unfold List.map. rewrite H. simpl. rewrite 
+
+
+ rewrite H8 in 
+
+
+ unfold Default. apply None. specialize (H1 _ _ _ (fun l : LPath b => snd (labelHead l)) _ _ _ _ H2 H4).
+      assert (h <> Heap.Empty) by (intro; subst). rewrite H1. simpl. rewrite H1.
+
+
+
+    destruct (Heap.isEmpty h) eqn : He. simpl.
+    destruct h. simpl in H0. destruct h'. simpl. reflexivity. simpl in H0; inversion H0. simpl in He; inversion He. simpl.
+    destruct (Heap.isEmpty h') eqn : Hf. destruct h'.
+
 
 Lemma dijkstra'_equiv: forall h g,
   dijkstra h g = dijkstra' (h, g).
@@ -390,7 +911,7 @@ Proof.
 Qed.
 
 (*Equivalence with tail recursive version*)
-Lemma leveln_tail_equiv: forall g h l,
+Lemma sp_tail_equiv: forall g h l,
   (forall k, ~In_Heap (k, LP nil) h) ->
   get_paths (sp_tail (g, h, l)) = l ++ dijkstra' (h, g).
 Proof.
